more renaming

theories/opsem.v
@@ -39,14 +39,14 @@ Inductive reduce_simple : seq administrative_instruction -> seq administrative_i
   (** testops **)
   | rs_testop_i32 :
     forall c testop,
-    reduce_simple [::AI_basic (BI_const (ConstInt32 c)); AI_basic (BI_testop T_i32 testop)] [::AI_basic (BI_const (ConstInt32 (wasm_bool (@app_testop_i i32t testop c))))]
+    reduce_simple [::AI_basic (BI_const (VAL_int32 c)); AI_basic (BI_testop T_i32 testop)] [::AI_basic (BI_const (VAL_int32 (wasm_bool (@app_testop_i i32t testop c))))]
   | rs_testop_i64 :
     forall c testop,
-    reduce_simple [::AI_basic (BI_const (ConstInt64 c)); AI_basic (BI_testop T_i64 testop)] [::AI_basic (BI_const (ConstInt32 (wasm_bool (@app_testop_i i64t testop c))))]
+    reduce_simple [::AI_basic (BI_const (VAL_int64 c)); AI_basic (BI_testop T_i64 testop)] [::AI_basic (BI_const (VAL_int32 (wasm_bool (@app_testop_i i64t testop c))))]
 
   (** relops **)
   | rs_relop: forall v1 v2 t op,
-    reduce_simple [::AI_basic (BI_const v1); AI_basic (BI_const v2); AI_basic (BI_relop t op)] [::AI_basic (BI_const (ConstInt32 (wasm_bool (app_relop op v1 v2))))]
+    reduce_simple [::AI_basic (BI_const v1); AI_basic (BI_const v2); AI_basic (BI_relop t op)] [::AI_basic (BI_const (VAL_int32 (wasm_bool (app_relop op v1 v2))))]
                     
   (** convert and reinterpret **)
   | rs_convert_success :
@@ -75,11 +75,11 @@ Inductive reduce_simple : seq administrative_instruction -> seq administrative_i
   | rs_select_false :
     forall n v1 v2,
     n = Wasm_int.int_zero i32m ->
-    reduce_simple [::AI_basic (BI_const v1); AI_basic (BI_const v2); AI_basic (BI_const (ConstInt32 n)); AI_basic BI_select] [::AI_basic (BI_const v2)]
+    reduce_simple [::AI_basic (BI_const v1); AI_basic (BI_const v2); AI_basic (BI_const (VAL_int32 n)); AI_basic BI_select] [::AI_basic (BI_const v2)]
   | rs_select_true :
     forall n v1 v2,
     n <> Wasm_int.int_zero i32m ->
-    reduce_simple [::AI_basic (BI_const v1); AI_basic (BI_const v2); AI_basic (BI_const (ConstInt32 n)); AI_basic BI_select] [::AI_basic (BI_const v1)]
+    reduce_simple [::AI_basic (BI_const v1); AI_basic (BI_const v2); AI_basic (BI_const (VAL_int32 n)); AI_basic BI_select] [::AI_basic (BI_const v1)]
   | rs_block :
       forall vs es n m t1s t2s,
         const_list vs ->
@@ -97,11 +97,11 @@ Inductive reduce_simple : seq administrative_instruction -> seq administrative_i
   | rs_if_false :
       forall n tf e1s e2s,
         n = Wasm_int.int_zero i32m ->
-        reduce_simple ([::AI_basic (BI_const (ConstInt32 n)); AI_basic (BI_if tf e1s e2s)]) [::AI_basic (BI_block tf e2s)]
+        reduce_simple ([::AI_basic (BI_const (VAL_int32 n)); AI_basic (BI_if tf e1s e2s)]) [::AI_basic (BI_block tf e2s)]
   | rs_if_true :
       forall n tf e1s e2s,
         n <> Wasm_int.int_zero i32m ->
-        reduce_simple ([::AI_basic (BI_const (ConstInt32 n)); AI_basic (BI_if tf e1s e2s)]) [::AI_basic (BI_block tf e1s)]
+        reduce_simple ([::AI_basic (BI_const (VAL_int32 n)); AI_basic (BI_if tf e1s e2s)]) [::AI_basic (BI_block tf e1s)]
   | rs_label_const :
       forall n es vs,
         const_list vs ->
@@ -118,20 +118,20 @@ Inductive reduce_simple : seq administrative_instruction -> seq administrative_i
   | rs_br_if_false :
       forall n i,
         n = Wasm_int.int_zero i32m ->
-        reduce_simple [::AI_basic (BI_const (ConstInt32 n)); AI_basic (BI_br_if i)] [::]
+        reduce_simple [::AI_basic (BI_const (VAL_int32 n)); AI_basic (BI_br_if i)] [::]
   | rs_br_if_true :
       forall n i,
         n <> Wasm_int.int_zero i32m ->
-        reduce_simple [::AI_basic (BI_const (ConstInt32 n)); AI_basic (BI_br_if i)] [::AI_basic (BI_br i)]
+        reduce_simple [::AI_basic (BI_const (VAL_int32 n)); AI_basic (BI_br_if i)] [::AI_basic (BI_br i)]
   | rs_br_table : (* ??? *)
       forall iss c i j,
         length iss > Wasm_int.nat_of_uint i32m c ->
         List.nth_error iss (Wasm_int.nat_of_uint i32m c) = Some j ->
-        reduce_simple [::AI_basic (BI_const (ConstInt32 c)); AI_basic (BI_br_table iss i)] [::AI_basic (BI_br j)]
+        reduce_simple [::AI_basic (BI_const (VAL_int32 c)); AI_basic (BI_br_table iss i)] [::AI_basic (BI_br j)]
   | rs_br_table_length :
       forall iss c i,
         length iss <= (Wasm_int.nat_of_uint i32m c) ->
-        reduce_simple [::AI_basic (BI_const (ConstInt32 c)); AI_basic (BI_br_table iss i)] [::AI_basic (BI_br i)]
+        reduce_simple [::AI_basic (BI_const (VAL_int32 c)); AI_basic (BI_br_table iss i)] [::AI_basic (BI_br i)]
   | rs_local_const :
       forall es n f,
         const_list es ->
@@ -172,16 +172,16 @@ Inductive reduce : store_record -> list value -> list administrative_instruction
       stab s i (Wasm_int.nat_of_uint i32m c) = Some cl ->
       stypes s i j = Some tf ->
       cl_type cl = tf ->
-      reduce s vs [::AI_basic (BI_const (ConstInt32 c)); AI_basic (Call_indirect j)] i s vs [::Invoke cl]
+      reduce s vs [::AI_basic (BI_const (VAL_int32 c)); AI_basic (Call_indirect j)] i s vs [::Invoke cl]
 | r_call_indirect_failure1 :
     forall s i j c cl vs,
       stab s i (Wasm_int.nat_of_uint i32m c) = Some cl ->
       stypes s i j <> Some (cl_type cl) ->
-      reduce s vs [::AI_basic (BI_const (ConstInt32 c)); AI_basic (Call_indirect j)] i s vs [::AI_trap]
+      reduce s vs [::AI_basic (BI_const (VAL_int32 c)); AI_basic (Call_indirect j)] i s vs [::AI_trap]
 | r_call_indirect_failure2 :
     forall s i j c vs,
       stab s i (Wasm_int.nat_of_uint i32m c) = None ->
-      reduce s vs [::AI_basic (BI_const (ConstInt32 c)); AI_basic (Call_indirect j)] i s vs [::AI_trap]
+      reduce s vs [::AI_basic (BI_const (VAL_int32 c)); AI_basic (Call_indirect j)] i s vs [::AI_trap]
 | r_invoke_native :
     forall cl t1s t2s ts es ves vcs n m k zs vs s i j,
       cl = Func_native j (Tf t1s t2s) ts es ->
@@ -230,72 +230,72 @@ Inductive reduce : store_record -> list value -> list administrative_instruction
       smem_ind s i = Some j ->
       List.nth_error s.(s_mems) j = Some m ->
       load m (Wasm_int.N_of_uint i32m k) off (t_length t) = Some bs ->
-      reduce s vs [::AI_basic (BI_const (ConstInt32 k)); AI_basic (Load t None a off)] i s vs [::AI_basic (BI_const (wasm_deserialise bs t))]
+      reduce s vs [::AI_basic (BI_const (VAL_int32 k)); AI_basic (Load t None a off)] i s vs [::AI_basic (BI_const (wasm_deserialise bs t))]
 | r_load_failure :
     forall s i t vs k a off m j,
       smem_ind s i = Some j ->
       List.nth_error s.(s_mems) j = Some m ->
       load m (Wasm_int.N_of_uint i32m k) off (t_length t) = None ->
-      reduce s vs [::AI_basic (BI_const (ConstInt32 k)); AI_basic (Load t None a off)] i s vs [::AI_trap]
+      reduce s vs [::AI_basic (BI_const (VAL_int32 k)); AI_basic (Load t None a off)] i s vs [::AI_trap]
 | r_load_packed_success :
     forall s i t tp vs k a off m j bs sx,
       smem_ind s i = Some j ->
       List.nth_error s.(s_mems) j = Some m ->
       load_packed sx m (Wasm_int.N_of_uint i32m k) off (tp_length tp) (t_length t) = Some bs ->
-      reduce s vs [::AI_basic (BI_const (ConstInt32 k)); AI_basic (Load t (Some (tp, sx)) a off)] i s vs [::AI_basic (BI_const (wasm_deserialise bs t))]
+      reduce s vs [::AI_basic (BI_const (VAL_int32 k)); AI_basic (Load t (Some (tp, sx)) a off)] i s vs [::AI_basic (BI_const (wasm_deserialise bs t))]
 | r_load_packed_failure :
     forall s i t tp vs k a off m j sx,
       smem_ind s i = Some j ->
       List.nth_error s.(s_mems) j = Some m ->
       load_packed sx m (Wasm_int.N_of_uint i32m k) off (tp_length tp) (t_length t) = None ->
-      reduce s vs [::AI_basic (BI_const (ConstInt32 k)); AI_basic (Load t (Some (tp, sx)) a off)] i s vs [::AI_trap]
+      reduce s vs [::AI_basic (BI_const (VAL_int32 k)); AI_basic (Load t (Some (tp, sx)) a off)] i s vs [::AI_trap]
 | r_store_success :
     forall t v s i j vs mem' k a off m,
       types_agree t v ->
       smem_ind s i = Some j ->
       List.nth_error s.(s_mems) j = Some m ->
       store m (Wasm_int.N_of_uint i32m k) off (bits v) (t_length t) = Some mem' ->
-      reduce s vs [::AI_basic (BI_const (ConstInt32 k)); AI_basic (BI_const v); AI_basic (Store t None a off)] i (upd_s_mem s (update_list_at s.(s_mems) j mem')) vs [::]
+      reduce s vs [::AI_basic (BI_const (VAL_int32 k)); AI_basic (BI_const v); AI_basic (Store t None a off)] i (upd_s_mem s (update_list_at s.(s_mems) j mem')) vs [::]
 | r_store_failure :
     forall t v s i j m k off a vs,
       types_agree t v ->
       smem_ind s i = Some j ->
       List.nth_error s.(s_mems) j = Some m ->
       store m (Wasm_int.N_of_uint i32m k) off (bits v) (t_length t) = None ->
-      reduce s vs [::AI_basic (BI_const (ConstInt32 k)); AI_basic (BI_const v); AI_basic (Store t None a off)] i s vs [::AI_trap]
+      reduce s vs [::AI_basic (BI_const (VAL_int32 k)); AI_basic (BI_const v); AI_basic (Store t None a off)] i s vs [::AI_trap]
 | r_store_packed_success :
     forall t v s i j m k off a vs mem' tp,
       types_agree t v ->
       smem_ind s i = Some j ->
       List.nth_error s.(s_mems) j = Some m ->
       store_packed m (Wasm_int.N_of_uint i32m k) off (bits v) (tp_length tp) = Some mem' ->
-      reduce s vs [::AI_basic (BI_const (ConstInt32 k)); AI_basic (BI_const v); AI_basic (Store t (Some tp) a off)] i (upd_s_mem s (update_list_at s.(s_mems) j mem')) vs [::]
+      reduce s vs [::AI_basic (BI_const (VAL_int32 k)); AI_basic (BI_const v); AI_basic (Store t (Some tp) a off)] i (upd_s_mem s (update_list_at s.(s_mems) j mem')) vs [::]
 | r_store_packed_failure :
     forall t v s i j m k off a vs tp,
       types_agree t v ->
       smem_ind s i = Some j ->
       List.nth_error s.(s_mems) j = Some m ->
       store_packed m (Wasm_int.N_of_uint i32m k) off (bits v) (tp_length tp) = None ->
-      reduce s vs [::AI_basic (BI_const (ConstInt32 k)); AI_basic (BI_const v); AI_basic (Store t (Some tp) a off)] i s vs [::AI_trap]
+      reduce s vs [::AI_basic (BI_const (VAL_int32 k)); AI_basic (BI_const v); AI_basic (Store t (Some tp) a off)] i s vs [::AI_trap]
 | r_current_memory :
     forall i j m n s vs,
       smem_ind s i = Some j ->
       List.nth_error s.(s_mems) j = Some m ->
       mem_size m = n ->
-      reduce s vs [::AI_basic (Current_memory)] i s vs [::AI_basic (BI_const (ConstInt32 (Wasm_int.int_of_Z i32m (Z.of_nat n))))]
+      reduce s vs [::AI_basic (Current_memory)] i s vs [::AI_basic (BI_const (VAL_int32 (Wasm_int.int_of_Z i32m (Z.of_nat n))))]
 | r_grow_memory_success :
     forall s i j m n mem' vs c,
       smem_ind s i = Some j ->
       List.nth_error s.(s_mems) j = Some m ->
       mem_size m = n ->
       mem_grow m (Wasm_int.N_of_uint i32m c) = Some mem' ->
-      reduce s vs [::AI_basic (BI_const (ConstInt32 c)); AI_basic Grow_memory] i (upd_s_mem s (update_list_at s.(s_mems) j mem')) vs [::AI_basic (BI_const (ConstInt32 (Wasm_int.int_of_Z i32m (Z.of_nat n))))]
+      reduce s vs [::AI_basic (BI_const (VAL_int32 c)); AI_basic Grow_memory] i (upd_s_mem s (update_list_at s.(s_mems) j mem')) vs [::AI_basic (BI_const (VAL_int32 (Wasm_int.int_of_Z i32m (Z.of_nat n))))]
 | r_grow_memory_failure :
     forall i j m n s vs c,
       smem_ind s i = Some j ->
       List.nth_error s.(s_mems) j = Some m ->
       mem_size m = n ->
-      reduce s vs [::AI_basic (BI_const (ConstInt32 c)); AI_basic Grow_memory] i s vs [::AI_basic (BI_const (ConstInt32 int32_minus_one))]
+      reduce s vs [::AI_basic (BI_const (VAL_int32 c)); AI_basic Grow_memory] i s vs [::AI_basic (BI_const (VAL_int32 int32_minus_one))]
 | r_label :
     forall s vs es les i s' vs' es' les' k lh,
       reduce s vs es i s' vs' es' ->
@@ -325,16 +325,16 @@ Inductive reduce : host_state -> store_record -> frame -> list administrative_in
         stab s f.(f_inst) (Wasm_int.nat_of_uint i32m c) = Some cl ->
         stypes s f.(f_inst) i = Some tf ->
         cl_type cl = tf ->
-        reduce hs s f [::AI_basic (BI_const (ConstInt32 c)); AI_basic (BI_call_indirect i)] hs s f [::AI_invoke cl]
+        reduce hs s f [::AI_basic (BI_const (VAL_int32 c)); AI_basic (BI_call_indirect i)] hs s f [::AI_invoke cl]
   | r_call_indirect_failure1 :
       forall s f i c cl hs,
         stab s f.(f_inst) (Wasm_int.nat_of_uint i32m c) = Some cl ->
         stypes s f.(f_inst) i <> Some (cl_type cl) ->
-        reduce hs s f [::AI_basic (BI_const (ConstInt32 c)); AI_basic (BI_call_indirect i)] hs s f [::AI_trap]
+        reduce hs s f [::AI_basic (BI_const (VAL_int32 c)); AI_basic (BI_call_indirect i)] hs s f [::AI_trap]
   | r_call_indirect_failure2 :
       forall s f i c hs,
         stab s f.(f_inst) (Wasm_int.nat_of_uint i32m c) = None ->
-        reduce hs s f [::AI_basic (BI_const (ConstInt32 c)); AI_basic (BI_call_indirect i)] hs s f [::AI_trap]
+        reduce hs s f [::AI_basic (BI_const (VAL_int32 c)); AI_basic (BI_call_indirect i)] hs s f [::AI_trap]
   | r_invoke_native :
       forall cl t1s t2s ts es ves vcs n m k zs s f f' i hs,
         cl = FC_func_native i (Tf t1s t2s) ts es ->
@@ -389,53 +389,53 @@ Inductive reduce : host_state -> store_record -> frame -> list administrative_in
       smem_ind s f.(f_inst) = Some i ->
       List.nth_error s.(s_mems) i = Some m ->
       load m (Wasm_int.N_of_uint i32m k) off (t_length t) = Some bs ->
-      reduce hs s f [::AI_basic (BI_const (ConstInt32 k)); AI_basic (BI_load t None a off)] hs s f [::AI_basic (BI_const (wasm_deserialise bs t))]
+      reduce hs s f [::AI_basic (BI_const (VAL_int32 k)); AI_basic (BI_load t None a off)] hs s f [::AI_basic (BI_const (wasm_deserialise bs t))]
   | r_load_failure :
     forall s i f t k a off m hs,
       smem_ind s f.(f_inst) = Some i ->
       List.nth_error s.(s_mems) i = Some m ->
       load m (Wasm_int.N_of_uint i32m k) off (t_length t) = None ->
-      reduce hs s f [::AI_basic (BI_const (ConstInt32 k)); AI_basic (BI_load t None a off)] hs s f [::AI_trap]
+      reduce hs s f [::AI_basic (BI_const (VAL_int32 k)); AI_basic (BI_load t None a off)] hs s f [::AI_trap]
   | r_load_packed_success :
     forall s i f t tp k a off m bs sx hs,
       smem_ind s f.(f_inst) = Some i ->
       List.nth_error s.(s_mems) i = Some m ->
       load_packed sx m (Wasm_int.N_of_uint i32m k) off (tp_length tp) (t_length t) = Some bs ->
-      reduce hs s f [::AI_basic (BI_const (ConstInt32 k)); AI_basic (BI_load t (Some (tp, sx)) a off)] hs s f [::AI_basic (BI_const (wasm_deserialise bs t))]
+      reduce hs s f [::AI_basic (BI_const (VAL_int32 k)); AI_basic (BI_load t (Some (tp, sx)) a off)] hs s f [::AI_basic (BI_const (wasm_deserialise bs t))]
   | r_load_packed_failure :
     forall s i f t tp k a off m sx hs,
       smem_ind s f.(f_inst) = Some i ->
       List.nth_error s.(s_mems) i = Some m ->
       load_packed sx m (Wasm_int.N_of_uint i32m k) off (tp_length tp) (t_length t) = None ->
-      reduce hs s f [::AI_basic (BI_const (ConstInt32 k)); AI_basic (BI_load t (Some (tp, sx)) a off)] hs s f [::AI_trap]
+      reduce hs s f [::AI_basic (BI_const (VAL_int32 k)); AI_basic (BI_load t (Some (tp, sx)) a off)] hs s f [::AI_trap]
   | r_store_success :
     forall t v s i f mem' k a off m hs,
       types_agree t v ->
       smem_ind s f.(f_inst) = Some i ->
       List.nth_error s.(s_mems) i = Some m ->
       store m (Wasm_int.N_of_uint i32m k) off (bits v) (t_length t) = Some mem' ->
-      reduce hs s f [::AI_basic (BI_const (ConstInt32 k)); AI_basic (BI_const v); AI_basic (BI_store t None a off)] hs (upd_s_mem s (update_list_at s.(s_mems) i mem')) f [::]
+      reduce hs s f [::AI_basic (BI_const (VAL_int32 k)); AI_basic (BI_const v); AI_basic (BI_store t None a off)] hs (upd_s_mem s (update_list_at s.(s_mems) i mem')) f [::]
   | r_store_failure :
     forall t v s i f m k off a hs,
       types_agree t v ->
       smem_ind s f.(f_inst) = Some i ->
       List.nth_error s.(s_mems) i = Some m ->
       store m (Wasm_int.N_of_uint i32m k) off (bits v) (t_length t) = None ->
-      reduce hs s f [::AI_basic (BI_const (ConstInt32 k)); AI_basic (BI_const v); AI_basic (BI_store t None a off)] hs s f [::AI_trap]
+      reduce hs s f [::AI_basic (BI_const (VAL_int32 k)); AI_basic (BI_const v); AI_basic (BI_store t None a off)] hs s f [::AI_trap]
   | r_store_packed_success :
     forall t v s i f m k off a mem' tp hs,
       types_agree t v ->
       smem_ind s f.(f_inst) = Some i ->
       List.nth_error s.(s_mems) i = Some m ->
       store_packed m (Wasm_int.N_of_uint i32m k) off (bits v) (tp_length tp) = Some mem' ->
-      reduce hs s f [::AI_basic (BI_const (ConstInt32 k)); AI_basic (BI_const v); AI_basic (BI_store t (Some tp) a off)] hs (upd_s_mem s (update_list_at s.(s_mems) i mem')) f [::]
+      reduce hs s f [::AI_basic (BI_const (VAL_int32 k)); AI_basic (BI_const v); AI_basic (BI_store t (Some tp) a off)] hs (upd_s_mem s (update_list_at s.(s_mems) i mem')) f [::]
   | r_store_packed_failure :
     forall t v s i f m k off a tp hs,
       types_agree t v ->
       smem_ind s f.(f_inst) = Some i ->
       List.nth_error s.(s_mems) i = Some m ->
       store_packed m (Wasm_int.N_of_uint i32m k) off (bits v) (tp_length tp) = None ->
-      reduce hs s f [::AI_basic (BI_const (ConstInt32 k)); AI_basic (BI_const v); AI_basic (BI_store t (Some tp) a off)] hs s f [::AI_trap]
+      reduce hs s f [::AI_basic (BI_const (VAL_int32 k)); AI_basic (BI_const v); AI_basic (BI_store t (Some tp) a off)] hs s f [::AI_trap]
 
   (** memory **)
   | r_current_memory :
@@ -443,20 +443,20 @@ Inductive reduce : host_state -> store_record -> frame -> list administrative_in
         smem_ind s f.(f_inst) = Some i ->
         List.nth_error s.(s_mems) i = Some m ->
         mem_size m = n ->
-        reduce hs s f [::AI_basic (BI_current_memory)] hs s f [::AI_basic (BI_const (ConstInt32 (Wasm_int.int_of_Z i32m (Z.of_nat n))))]
+        reduce hs s f [::AI_basic (BI_current_memory)] hs s f [::AI_basic (BI_const (VAL_int32 (Wasm_int.int_of_Z i32m (Z.of_nat n))))]
   | r_grow_memory_success :
     forall s i f m n mem' c hs,
       smem_ind s f.(f_inst) = Some i ->
       List.nth_error s.(s_mems) i = Some m ->
       mem_size m = n ->
       mem_grow m (Wasm_int.N_of_uint i32m c) = Some mem' ->
-      reduce hs s f [::AI_basic (BI_const (ConstInt32 c)); AI_basic BI_grow_memory] hs (upd_s_mem s (update_list_at s.(s_mems) i mem')) f [::AI_basic (BI_const (ConstInt32 (Wasm_int.int_of_Z i32m (Z.of_nat n))))]
+      reduce hs s f [::AI_basic (BI_const (VAL_int32 c)); AI_basic BI_grow_memory] hs (upd_s_mem s (update_list_at s.(s_mems) i mem')) f [::AI_basic (BI_const (VAL_int32 (Wasm_int.int_of_Z i32m (Z.of_nat n))))]
   | r_grow_memory_failure :
       forall i f m n s c hs,
         smem_ind s f.(f_inst) = Some i ->
         List.nth_error s.(s_mems) i = Some m ->
         mem_size m = n ->
-        reduce hs s f [::AI_basic (BI_const (ConstInt32 c)); AI_basic BI_grow_memory] hs s f [::AI_basic (BI_const (ConstInt32 int32_minus_one))]
+        reduce hs s f [::AI_basic (BI_const (VAL_int32 c)); AI_basic BI_grow_memory] hs s f [::AI_basic (BI_const (VAL_int32 int32_minus_one))]
 
   (** label and local **)
   | r_label :
