theories/pp.v
@@ -134,10 +134,10 @@ Definition pp_f64 (f : float) : string :=
 
 Definition pp_value (v : value) : string :=
   match v with
-  | ConstInt32 i => pp_value_type T_i32 ++ ".const " ++ with_fg FG_green (pp_i32 i) ++ newline
-  | ConstInt64 i => pp_value_type T_i64 ++ ".const " ++ with_fg FG_green (pp_i64 i) ++ newline
-  | ConstFloat32 f => pp_value_type T_f32 ++ ".const " ++ with_fg FG_green (pp_f32 f) ++ newline
-  | ConstFloat64 f => pp_value_type T_f64 ++ ".const " ++ with_fg FG_green (pp_f64 f) ++ newline
+  | VAL_int32 i => pp_value_type T_i32 ++ ".const " ++ with_fg FG_green (pp_i32 i) ++ newline
+  | VAL_int64 i => pp_value_type T_i64 ++ ".const " ++ with_fg FG_green (pp_i64 i) ++ newline
+  | VAL_float32 f => pp_value_type T_f32 ++ ".const " ++ with_fg FG_green (pp_f32 f) ++ newline
+  | VAL_float64 f => pp_value_type T_f64 ++ ".const " ++ with_fg FG_green (pp_f64 f) ++ newline
   end.
 
 Definition pp_values (vs : list value) : string :=
