theories/type_progress.v
@@ -783,7 +783,7 @@ Proof.
     eapply mem_context_store in H; eauto.
     destruct H as [n [HMemInd HMem]].
     destruct (List.nth_error (s_mems s) n) eqn:HN => //=.
-    exists s, f, [::AI_basic (BI_const (ConstInt32 (Wasm_int.int_of_Z i32m (Z.of_nat (mem_size m)))))], hs.
+    exists s, f, [::AI_basic (BI_const (VAL_int32 (Wasm_int.int_of_Z i32m (Z.of_nat (mem_size m)))))], hs.
     by eapply r_current_memory; eauto.
 
   - (* Grow_memory *)
@@ -794,7 +794,7 @@ Proof.
     destruct (List.nth_error (s_mems s) n) eqn:HN => //=.
     destruct v => //=.
     (* Similarly, for this proof we can just use trap and use the failure case. *)
-    exists s, f, [::AI_basic (BI_const (ConstInt32 int32_minus_one))], hs.
+    exists s, f, [::AI_basic (BI_const (VAL_int32 int32_minus_one))], hs.
     by eapply r_grow_memory_failure; eauto.
 
   - (* Composition *)
